List remaining bvp_to_word ops, start on WordShift w8
It looks like the semantics of WordShift might need to change,
though, to restrict the size of the shift to the word size or less.
(This could be at the source level, or in compilation into bvl.)

compiler/backend/bvp_to_wordScript.sml
@@ -127,6 +127,7 @@ val assign_def = Define `
     | Global _ => (Skip,l)
     | SetGlobal _ => (Skip,l)
     | AllocGlobal => (Skip,l)
+    (* TODO: FromList *)
     | El => (case args of
              | [v1;v2] => (Assign (adjust_var dest)
                             (Load (Op Add [real_addr c (adjust_var v1);
@@ -154,6 +155,7 @@ val assign_def = Define `
                              (adjust_var v3))
                       (Assign (adjust_var dest) Unit),l)
              | _ => (Skip,l))
+    (* TODO: UpdateByte *)
     | Cons tag => if LENGTH args = 0 then
                     if tag < dimword (:'a) DIV 16 then
                       (Assign (adjust_var dest) (Const (n2w (16 * tag + 2))),l)
@@ -185,6 +187,8 @@ val assign_def = Define `
                     (Op Or [Shift Lsl (Op Sub [Var 1; Lookup CurrHeap])
                               (Nat (shift_length c − shift (:'a)));
                             Const 1w])],l))
+    (* TODO: RefByte *)
+    (* TODO: RefArray *)
     | Label n => (LocValue (adjust_var dest) (2 * n + bvl_to_bvi$num_stubs) 0,l)
     | Equal => (case args of
                | [v1;v2] =>
@@ -334,6 +338,9 @@ val assign_def = Define `
                                       Var (adjust_var v2)]))
                           GiveUp),l)
               | _ => (Skip,l))
+    (* TODO: Mult *)
+    (* TODO: Div *)
+    (* TODO: Mod *)
     | WordOp W8 opw =>
       (case args of
         | [v1;v2] =>
@@ -382,6 +389,39 @@ val assign_def = Define `
                             (Nat (shift_length c − shift (:'a)));
                           Const 1w])], l))
        | _ => (Skip,l))
+    (* TODO: semantics of WordShift needs to limit n to the word size
+    | WordShift W8 sh n => (case args of
+      | [v1] =>
+        (Assign (adjust_var dest)
+           (case sh of
+            | Lsl =>
+              Shift Lsr
+                (Shift Lsl (Var (adjust_var v1)) (Nat (dimindex(:'a) - 10 + n)))
+                (Nat (dimindex(:'a) - 10))
+            | Lsr =>
+              Shift Lsl
+                (Shift Lsr (Var (adjust_var v1)) (Nat (n+2)))
+                (Nat 2)
+            | Asr =>
+              Shift Lsl
+                (Shift Lsr
+                   (Shift Asr
+                      (Shift Lsl (Var (adjust_var v1)) (Nat (dimindex(:'a) - 10)))
+                      (Nat n))
+                   (Nat (dimindex(:'a) - 8)))
+                (Nat 2))
+        ,l)
+      | _ => (GiveUp,l)) *)
+    (* TODO: WordShift W64 *)
+    (* TODO:
+    | WordFromInt => (case args of
+      | [v1] =>
+        let len = if dimindex(:'a) < 64 then 2 else 1 in
+        (case encode_header c 3 len of
+         | NONE => (GiveUp,l)
+         | SOME (header:'a word) => ...)
+      | _ => (Skip, l)) *)
+    (* TODO: WordToInt *)
     | FFI ffi_index =>
       (case args of
        | [v] =>
